refactor: use Program instead of refine

src/x86/Architecture/MemoryController/MemoryController_eq.v
@@ -1,13 +1,16 @@
+Require Import Coq.Program.Tactics.
+
 Require Import SpecCert.Utils.
 Require Import SpecCert.x86.Architecture.MemoryController.MemoryController_rec.
 
-Definition memory_controller_eq (m m':MemoryController) :=
+Definition memory_controller_eq
+           (m m': MemoryController) :=
   smramc m = smramc m'.
 
-Lemma memory_controller_eq_eq: forall m m':MemoryController,
-  memory_controller_eq m m' -> m = m'.
+Lemma memory_controller_eq_eq
+      (m m': MemoryController)
+  : memory_controller_eq m m' -> m = m'.
 Proof.
-  intros m m'.
   induction m as [s].
   induction m' as [s'].
   unfold memory_controller_eq, smramc.
@@ -16,32 +19,31 @@ Proof.
   reflexivity.
 Qed.
 
-Lemma eq_memory_controller_eq: forall m m':MemoryController,
-  m = m' -> memory_controller_eq m m'.
+Lemma eq_memory_controller_eq
+      (m m': MemoryController)
+      (Heq:  m = m')
+  : memory_controller_eq m m'.
 Proof.
-  intros m m'.
   induction m as [s].
   induction m' as [s'].
-  intro Heq.
   rewrite Heq.
   reflexivity.
 Qed.
 
-Definition memory_controller_eq_dec (m m':MemoryController):
-  {memory_controller_eq m m'}+{~memory_controller_eq m m'}.
-refine (
-  decide_dec (smramc_eq_dec (smramc m) (smramc m'))
-).
-+ unfold memory_controller_eq.
+Program Definition memory_controller_eq_dec
+        (m m': MemoryController)
+  : { memory_controller_eq m m' } + { ~ memory_controller_eq m m' } :=
+  decide_dec (smramc_eq_dec (smramc m) (smramc m')).
+Next Obligation.
+  unfold memory_controller_eq.
   apply smramc_eq_eq.
   trivial.
-+ unfold memory_controller_eq.
-  unfold not in n; unfold not.
+Defined.
+Next Obligation.
+  unfold memory_controller_eq.
+  unfold not in H; unfold not.
   intro Hfalse.
   apply eq_smramc_eq in Hfalse.
-  apply n in Hfalse.
+  apply H in Hfalse.
   trivial.
 Defined.
-
-Definition memory_controller_eqb (m m':MemoryController) :=
-  if memory_controller_eq_dec m m' then true else false.
