src/Address/HardwareAddress.v
@@ -71,7 +71,7 @@ Definition is_vga (ha:HardwareAddress) :=
   address_scope ha = VGA.
 
 Definition is_same_memory (ha ha':HardwareAddress) :=
-  (is_dram ha /\ is_dram ha') \/ (is_vga ha /\ is_vga ha').
+  address_scope ha = address_scope ha'.
 
 (**
    Decidable Properties
@@ -85,38 +85,20 @@ Defined.
 
 Definition hardware_addr_eq_dec
            (ha ha': HardwareAddress)
-  : {addr_eq ha ha'}+{~ addr_eq ha ha'}.
-refine (decide_dec (addr_eq_dec ha ha')); trivial.
-Defined.
+  : { addr_eq ha ha' } + { ~ addr_eq ha ha' } :=
+  addr_eq_dec ha ha'.
 
-Definition is_dram_dec (ha:HardwareAddress)
-  :{is_dram ha}+{~is_dram ha}.
-refine (
-    decide_dec (scope_eq_dec (address_scope ha) DRAM)); unfold is_dram;
-  [ exact e
-  | exact n ].
-Defined.
+Definition is_dram_dec
+           (ha: HardwareAddress)
+  : { is_dram ha } + { ~ is_dram ha } :=
+  scope_eq_dec (address_scope ha) DRAM.
 
-Definition is_vga_dec (ha:HardwareAddress)
-  :{is_vga ha}+{~is_vga ha}.
-refine (
-    decide_dec (scope_eq_dec (address_scope ha) VGA)); unfold is_dram;
-  [ exact e
-  | exact n ].
-Defined.
+Definition is_vga_dec
+           (ha: HardwareAddress)
+  : { is_vga ha } + { ~ is_vga ha } :=
+  scope_eq_dec (address_scope ha) VGA.
 
-Definition is_same_memory_dec (ha ha':HardwareAddress)
-  : {is_same_memory ha ha'}+{~is_same_memory ha ha'}.
-refine(
-  decide_dec (
-    sumbool_or _ _ _ _ (sumbool_and _ _ _ _ (is_dram_dec ha)
-                                            (is_dram_dec ha')
-                       )
-                       (sumbool_and _ _ _ _ (is_vga_dec ha)
-                                            (is_vga_dec ha')
-                       )
-  )
-); unfold is_same_memory; trivial.
-inversion a.
-apply and_not_or; split; apply or_not_and; trivial.
-Defined.
+Program Definition is_same_memory_dec
+        (ha ha': HardwareAddress)
+  : { is_same_memory ha ha' } + { ~ is_same_memory ha ha' } :=
+  decide_dec (scope_eq_dec (address_scope ha) (address_scope ha')).
