src/Interval/Interval_dec.v
@@ -1,39 +1,58 @@
 Require Import Coq.Bool.Sumbool.
 Require Import Coq.Arith.Compare_dec.
+Require Import Omega.
 
 Require Import SpecCert.Interval.Interval_ind.
 Require Import SpecCert.Interval.Interval_func.
 Require Import SpecCert.Interval.Interval_prop.
 Require Import SpecCert.Utils.
 
-Definition is_inside_interval_dec (x:nat)(i:Interval)
-  :{is_inside_interval x i}+{~is_inside_interval x i}. 
-Proof.
-  refine (
+Program Definition is_inside_interval_dec
+        (x: nat)
+        (i: Interval)
+  :{ is_inside_interval x i } + { ~ is_inside_interval x i } :=
     let b := lower_bound i in
     let e := upper_bound i in
-      decide_dec (sumbool_and _ _ _ _ (le_dec b x) (le_dec x e))
-  ); unfold is_inside_interval; intuition.
-Defined.
+    (le_dec b x) :&& (le_dec x e).
+Next Obligation.
+  unfold is_inside_interval.
+  omega.
+Qed.
+Next Obligation.
+  unfold is_inside_interval.
+  omega.
+Qed.
 
-Definition is_included_dec (i1 i2:Interval)
-  :{is_included_in i1 i2}+{~is_included_in i1 i2}.
-Proof.
-  refine (
+Program Definition is_included_dec
+        (i1 i2: Interval)
+  : { is_included_in i1 i2 } + { ~ is_included_in i1 i2 } :=
   let b1 := lower_bound i1 in
   let b2 := lower_bound i2 in
   let e2 := upper_bound i2 in
   let e1 := upper_bound i1 in
-    decide_dec (sumbool_and _ _ _ _ (le_dec b2 b1) (le_dec e1 e2))
-  ); unfold is_included_in; intuition.
-Defined.
+  (le_dec b2 b1) :&& (le_dec e1 e2).
+Next Obligation.
+  unfold is_included_in.
+  omega.
+Qed.
+Next Obligation.
+  unfold is_included_in.
+  omega.
+Qed.
 
-Definition disjoint_dec (i1 i2:Interval): {disjoint i1 i2}+{~disjoint i1 i2}.
-refine (
+Program Definition disjoint_dec
+        (i1 i2: Interval)
+  : { disjoint i1 i2 } + { ~ disjoint i1 i2 } :=
   let b1 := lower_bound i1 in
   let b2 := lower_bound i2 in
   let e1 := upper_bound i1 in
   let e2 := upper_bound i2 in
-  decide_dec (sumbool_and _ _ _ _ (lt_dec e1 b2) (lt_dec e2 b1))
-); unfold disjoint; simpl; intuition.
-Defined.
+  (lt_dec e1 b2) :&& (lt_dec e2 b1).
+Next Obligation.
+  unfold disjoint.
+  omega.
+Qed.
+Next Obligation.
+  unfold disjoint.
+  omega.
+Qed.
