src/x86/Architecture/MemoryController/MemoryController_func.v
@@ -1,40 +1,34 @@
+Require Import Coq.Program.Tactics.
+
 Require Import SpecCert.x86.Architecture.MemoryController.Registers.
 Require Import SpecCert.x86.Architecture.MemoryController.MemoryController_rec.
 Require Import SpecCert.x86.Architecture.MemoryController.MemoryController_prop.
 Require Import SpecCert.x86.Architecture.MemoryController.MemoryController_dec.
 Require Import SpecCert.Address.
 
-Definition open_smram
-           (mc :MemoryController)
-           (h  :smramc_is_unlocked mc)
-           :MemoryController.
-refine (
-  {| smramc := set_d_open (smramc mc) _ |}
-).
-unfold smramc_is_unlocked in h; trivial.
-Defined.
+Program Definition open_smram
+        (mc: MemoryController)
+        (h:  smramc_is_unlocked mc)
+  : MemoryController :=
+  {| smramc := set_d_open (smramc mc) _ |}.
 
-Definition close_smram (mc:MemoryController)
-                       (h:smramc_is_unlocked mc):MemoryController.
-refine (
-  {| smramc := unset_d_open (smramc mc) _ |}
-).
-unfold smramc_is_unlocked in h; trivial.
-Defined.
+Program Definition close_smram
+        (mc: MemoryController)
+        (h:  smramc_is_unlocked mc)
+  : MemoryController :=
+  {| smramc := unset_d_open (smramc mc) _ |}.
 
-Definition lock_smramc (mc:MemoryController)
-                       (h:smramc_is_unlocked mc):MemoryController.
-refine (
-  {| smramc := set_d_lock (smramc mc) _ |}
-).
-unfold smramc_is_unlocked in h; trivial.
-Defined.
+Program Definition lock_smramc
+        (mc: MemoryController)
+        (h:  smramc_is_unlocked mc)
+  : MemoryController :=
+  {| smramc := set_d_lock (smramc mc) _ |}.
 
 Definition translate_physical_address
-           (mc     :MemoryController)
-           (smiact :bool)
-           (pa     :PhysicalAddress)
-           :HardwareAddress :=
+           (mc:     MemoryController)
+           (smiact: bool)
+           (pa:     PhysicalAddress)
+  : HardwareAddress :=
   if is_inside_smram_dec pa then
     if can_access_smram_dec mc smiact then
       dram pa
